src/paths-new/Binding.v
@@ -1,0 +1,1130 @@
+(** printing ⊢#    %\vdash_{\#}%    #&vdash;<sub>&#35;</sub>#     *)
+(** printing ⊢##   %\vdash_{\#\#}%  #&vdash;<sub>&#35&#35</sub>#  *)
+(** printing ⊢##v  %\vdash_{\#\#v}% #&vdash;<sub>&#35&#35v</sub># *)
+(** printing ⊢!    %\vdash_!%       #&vdash;<sub>!</sub>#         *)
+(** remove printing ~ *)
+
+(** This module defines various helper lemmas about opening, closing, and local closure. *)
+
+Set Implicit Arguments.
+
+Require Import Coq.Program.Equality List.
+Require Import LibLN.
+Require Import Definitions Helper_lemmas.
+
+
+(** Substitution on variables: [a[u/z]] (substituting [z] with [u] in [a]). *)
+
+Definition subst_var (z: var) (u: var) (x: var): var :=
+  If x = z then u else x.
+
+Definition subst_var_p (z: var) (u: path) (x: var): path :=
+  If x = z then u else (pvar x).
+
+Hint Unfold subst_var subst_var_p.
+
+Definition subst_avar (z: var) (u: path) (a: avar) : path :=
+  match a with
+  | avar_b i => p_sel (avar_b i) nil
+  | avar_f x => subst_var_p z u x
+  end.
+
+(* p    [u / z] where p = x.bs:
+   x.bs [u / z] == x [u / z] . bs *)
+Definition subst_path (z: var) (u: path) (p: path) : path :=
+  match p with
+  | p_sel x bs => sel_fields (subst_avar z u x) bs
+  end.
+
+(** Substitution on types and declarations: [T[u/z]] and [D[u/z]]. *)
+Fixpoint subst_typ (z: var) (u: path) (T: typ) { struct T } : typ :=
+  match T with
+  | typ_top        => typ_top
+  | typ_bot        => typ_bot
+  | typ_rcd D      => typ_rcd (subst_dec z u D)
+  | typ_and T1 T2  => typ_and (subst_typ z u T1) (subst_typ z u T2)
+  | typ_path q L    => typ_path (subst_path z u q) L
+  | typ_bnd T      => typ_bnd (subst_typ z u T)
+  | typ_all T U    => typ_all (subst_typ z u T) (subst_typ z u U)
+  end
+with subst_dec (z: var) (u: path) (D: dec) { struct D } : dec :=
+  match D with
+  | dec_typ L T U => dec_typ L (subst_typ z u T) (subst_typ z u U)
+  | dec_trm L U => dec_trm L (subst_typ z u U)
+  end.
+
+(** Substitution on terms, values, and definitions:
+    [t[u/z]], [v[u/z]], [d[u/z]]. *)
+Fixpoint subst_trm (z: var) (u: path) (t: trm) : trm :=
+  match t with
+  | trm_val v        => trm_val (subst_val z u v)
+  | trm_path p       => trm_path (subst_path z u p)
+  | trm_app x1 x2    => trm_app (subst_path z u x1) (subst_path z u x2)
+  | trm_let t1 t2    => trm_let (subst_trm z u t1) (subst_trm z u t2)
+  end
+with subst_val (z: var) (u: path) (v: val) : val :=
+  match v with
+  | val_new T ds     => val_new (subst_typ z u T) (subst_defs z u ds)
+  | val_lambda T t   => val_lambda (subst_typ z u T) (subst_trm z u t)
+  end
+with subst_def (z: var) (u: path) (d: def) : def :=
+  match d with
+  | def_typ L T => def_typ L (subst_typ z u T)
+  | def_trm L t => def_trm L (subst_trm z u t)
+  end
+with subst_defs (z: var) (u: path) (ds: defs) : defs :=
+  match ds with
+  | defs_nil => defs_nil
+  | defs_cons rest d => defs_cons (subst_defs z u rest) (subst_def z u d)
+  end.
+
+(** Substitution on the types of a typing environment: [G[u/z]]. *)
+Definition subst_ctx (z: var) (u: path) (G: ctx) : ctx :=
+  map (subst_typ z u) G.
+
+(** * Lemmas *)
+
+(** The following [subst_fresh_XYZ] lemmas state that if [x] is not free
+    in a symbol [Y], then [Y[z/x] = Y]. *)
+
+(** Substitution on the values of an evaluation context: [e[y/x]]. *)
+Definition subst_env x y e := map (subst_val x y) e.
+
+
+(** * Opening Lemmas *)
+
+Ltac avar_solve :=
+  repeat match goal with
+  | [ a: avar |- _ ] =>
+    destruct a; simpl; auto; repeat case_if; subst; simpls; repeat case_if*;
+    subst; simpls; repeat case_if*
+  end.
+
+(** The following [open_fresh_XYZ_injective] lemmas state that given two
+    symbols (variables, types, terms, etc.) [X] and [Y] and a variable [z],
+    if [z \notin fv(X)] and [z \notin fv(Y)], then [X^z = Y^z] implies [X = Y]. *)
+
+(** - variables *)
+Lemma open_fresh_avar_injective : forall x y k z,
+    z \notin fv_avar x ->
+    z \notin fv_avar y ->
+    open_rec_avar k z x = open_rec_avar k z y ->
+    x = y.
+Proof.
+  intros. avar_solve; inversion* H1; try (inversions H3; false* notin_same).
+Qed.
+
+(** The following [lc_open_rec_open_XYZ] lemmas state that if opening
+    a symbol (variables, types, terms, etc.) at index [n] that is
+    already opened at index [m] results in the same opened symbol,
+    opening the symbol itself at index [n] results in the same symbol. *)
+
+
+(** - types and declarations *)
+Lemma lc_open_rec_open_typ_dec: forall x y,
+    (forall T n m,
+        n <> m ->
+        open_rec_typ n x (open_rec_typ m y T) = open_rec_typ m y T ->
+        open_rec_typ n x T = T) /\
+    (forall D n m,
+        n <> m ->
+        open_rec_dec n x (open_rec_dec m y D) = open_rec_dec m y D ->
+        open_rec_dec n x D = D).
+Proof.
+  introv. apply typ_mutind; intros; simpls; auto; avar_solve;
+            try solve [(inversions H1; erewrite H; eauto)
+                      || (inversions H2; erewrite H; eauto; erewrite H0; eauto)]. Admitted. (*
+  - inversions H1. rewrite H with (m:=S m); auto.
+  - inversions H2. erewrite H; eauto. rewrite H0 with (m:=S m); auto.
+Qed.*)
+
+(** - terms, values, definitions, and list of definitions *)
+Lemma lc_open_rec_open_trm_val_def_defs: forall x y,
+    (forall t n m,
+        n <> m ->
+        open_rec_trm n x (open_rec_trm m y t) = open_rec_trm m y t ->
+        open_rec_trm n x t = t) /\
+    (forall v n m,
+        n <> m ->
+        open_rec_val n x (open_rec_val m y v) = open_rec_val m y v ->
+        open_rec_val n x v = v) /\
+    (forall d n m,
+        n <> m ->
+        open_rec_def n x (open_rec_def m y d) = open_rec_def m y d ->
+        open_rec_def n x d = d) /\
+    (forall ds n m,
+        n <> m ->
+        open_rec_defs n x (open_rec_defs m y ds) = open_rec_defs m y ds ->
+        open_rec_defs n x ds = ds).
+Proof.
+  intros.
+  pose proof (proj21 (lc_open_rec_open_typ_dec x y)) as Htyp.
+  apply trm_mutind;
+    intros; simpls; auto;
+      match goal with
+      | [ H : _ = _ |- _ ] => injection H as ?; f_equal; eauto
+      end; avar_solve.
+Admitted.
+
+(** [x \notin fv(x, y)] #<br>#
+    [―――――――――――――――――] #<br>#
+    [x \notin fv(x^y)] *)
+Lemma open_fv_avar : forall x z y k,
+    x \notin fv_avar z \u \{y} ->
+    x \notin fv_avar (open_rec_avar k y z).
+Proof.
+  intros. destruct z; simpls; try case_if; unfold fv_avar; auto.
+Qed.
+
+(** [x \notin fv(T, y)] #<br>#
+    [―――――――――――――――――] #<br>#
+    [x \notin fv(T^y)] *)
+Lemma open_fv_typ_dec :
+  (forall T x y k, x \notin fv_typ T \u \{y} -> x \notin fv_typ (open_rec_typ k y T)) /\
+  (forall D x y k, x \notin fv_dec D \u \{y} -> x \notin fv_dec (open_rec_dec k y D)).
+Proof. Admitted. (*
+  apply typ_mutind; intros; simpls; auto;
+    apply open_fv_avar; auto.
+Qed.*)
+
+(** [x \notin fv(t, y)] #<br>#
+    [―――――――――――――――――] #<br>#
+    [x \notin fv(t^y)] *)
+Lemma open_fv_trm_val_def_defs :
+  (forall t x y k, x \notin fv_trm t \u \{y} -> x \notin fv_trm (open_rec_trm k y t)) /\
+  (forall v x y k, x \notin fv_val v \u \{y} -> x \notin fv_val (open_rec_val k y v)) /\
+  (forall d x y k, x \notin fv_def d \u \{y} -> x \notin fv_def (open_rec_def k y d)) /\
+  (forall ds x y k, x \notin fv_defs ds \u \{y} -> x \notin fv_defs (open_rec_defs k y ds)).
+Proof.
+  Local Hint Resolve open_fv_avar.
+  apply trm_mutind; intros; simpls; auto;
+    try apply notin_union_l;
+    try apply open_fv_typ_dec; auto. Admitted.
+
+
+(** * Local Closure
+
+  Our definition of [trm] accepts terms that contain de Bruijn indices that are unbound.
+  A symbol [X] is considered locally closed, denoted [lc X], if all de Bruijn indices
+  in [X] are bound.
+   We will require a term to be locally closed in the final safety theorem. *)
+
+(** Only named variables are locally closed. *)
+Inductive lc_at_var (k : nat) : avar -> Prop :=
+| lc_at_f : forall x, lc_at_var k (avar_f x)
+| lc_at_b : forall i, i < k -> lc_at_var k (avar_b i).
+Hint Constructors lc_at_var.
+
+Inductive lc_at_path (k: nat) : path -> Prop :=
+| lc_at_p : forall x bs, lc_at_var k x -> lc_at_path k (p_sel x bs).
+Hint Constructors lc_at_path.
+
+(** Locally closed types and declarations. *)
+Inductive lc_at_typ (k : nat) : typ -> Prop :=
+| lc_at_typ_top : lc_at_typ k typ_top
+| lc_at_typ_bot : lc_at_typ k typ_bot
+| lc_at_typ_rcd : forall D,
+    lc_at_dec k D ->
+    lc_at_typ k (typ_rcd D)
+| lc_at_typ_and : forall T1 T2,
+    lc_at_typ k T1 ->
+    lc_at_typ k T2 ->
+    lc_at_typ k (typ_and T1 T2)
+| lc_at_typ_sel : forall x L,
+    lc_at_path k x ->
+    lc_at_typ k (typ_path x L)
+| lc_at_typ_bnd : forall T,
+    lc_at_typ (S k) T ->
+    lc_at_typ k (typ_bnd T)
+| lc_at_typ_all : forall T1 T2,
+    lc_at_typ (S k) T2 ->
+    lc_at_typ k T1 ->
+    lc_at_typ k (typ_all T1 T2)
+with lc_at_dec (k : nat) : dec -> Prop :=
+| lc_at_dec_typ : forall L T U,
+    lc_at_typ k T ->
+    lc_at_typ k U ->
+    lc_at_dec k (dec_typ L T U)
+| lc_at_dec_trm : forall a T,
+    lc_at_typ k T ->
+    lc_at_dec k (dec_trm a T).
+Hint Constructors lc_at_typ lc_at_dec.
+
+
+(** Locally closed terms, values, and definitions. *)
+Inductive lc_at_trm (k : nat) : trm -> Prop :=
+| lc_at_trm_path : forall p,
+    lc_at_path k p ->
+    lc_at_trm k (trm_path p)
+| lc_at_trm_val : forall v,
+    lc_at_val k v ->
+    lc_at_trm k (trm_val v)
+| lc_at_trm_app : forall f a,
+    lc_at_path k f ->
+    lc_at_path k a ->
+    lc_at_trm k (trm_app f a)
+| lc_at_trm_let : forall t1 t2,
+    lc_at_trm k t1 ->
+    lc_at_trm (S k) t2 ->
+    lc_at_trm k (trm_let t1 t2)
+with lc_at_val (k : nat) : val -> Prop :=
+| lc_at_val_new : forall T ds,
+    lc_at_typ (S k) T ->
+    lc_at_defs (S k) ds ->
+    lc_at_val k (val_new T ds)
+| lc_at_val_lam : forall T t,
+    lc_at_typ k T ->
+    lc_at_trm (S k) t ->
+    lc_at_val k (val_lambda T t)
+with lc_at_def (k : nat) : def -> Prop :=
+| lc_at_def_typ : forall L T,
+    lc_at_typ k T ->
+    lc_at_def k (def_typ L T)
+| lc_at_def_trm : forall a t,
+    lc_at_trm k t ->
+    lc_at_def k (def_trm a t)
+with lc_at_defs (k : nat) : defs -> Prop :=
+| lc_at_defs_nil : lc_at_defs k defs_nil
+| lc_at_defs_cons : forall ds d,
+    lc_at_defs k ds ->
+    lc_at_def k d ->
+    lc_at_defs k (defs_cons ds d).
+Hint Constructors lc_at_trm lc_at_val lc_at_def lc_at_defs.
+
+
+Notation "'lc_var' x" := (lc_at_var 0 x) (at level 0).
+Notation "'lc_path' p" := (lc_at_path 0 p) (at level 0).
+Notation "'lc_typ' T" := (lc_at_typ 0 T) (at level 0).
+Notation "'lc_dec' D" := (lc_at_dec 0 D) (at level 0).
+
+Notation "'lc_trm' t" := (lc_at_trm 0 t) (at level 0).
+Notation "'lc_val' v" := (lc_at_val 0 v) (at level 0).
+Notation "'lc_def' d" := (lc_at_def 0 d) (at level 0).
+Notation "'lc_defs' ds" := (lc_at_defs 0 ds) (at level 0).
+
+
+Scheme lc_at_trm_mut  := Induction for lc_at_trm Sort Prop
+with   lc_at_val_mut  := Induction for lc_at_val Sort Prop
+with   lc_at_def_mut  := Induction for lc_at_def Sort Prop
+with   lc_at_defs_mut := Induction for lc_at_defs Sort Prop.
+Combined Scheme lc_at_mutind from lc_at_trm_mut, lc_at_val_mut, lc_at_def_mut, lc_at_defs_mut.
+
+Scheme lc_at_typ_mut := Induction for lc_at_typ Sort Prop
+with   lc_at_dec_mut := Induction for lc_at_dec Sort Prop.
+Combined Scheme lc_at_typ_mutind from lc_at_typ_mut, lc_at_dec_mut.
+
+
+(** Locally closed evaluation contexts *)
+Inductive lc_ec : ec -> Prop :=
+| lc_ec_empty : lc_ec empty
+| lc_ec_cons : forall x v e,
+    lc_ec e ->
+    lc_val v ->
+    lc_ec (e & x ~ v).
+Hint Constructors lc_ec.
+
+(** ** Local Closure Lemmas *)
+
+Lemma lc_at_relaxing_typ_dec :
+    (forall T k j, lc_at_typ k T -> j >= k -> lc_at_typ j T) /\
+    (forall D k j, lc_at_dec k D -> j >= k -> lc_at_dec j D).
+Proof with auto. Admitted. (*
+  apply typ_mutind; intros; simpl; auto;
+    match goal with
+    | [ H : lc_at_typ _ _ |- _ ] => inversions H
+    | [ H : lc_at_dec _ _ |- _ ] => inversions H
+    end;
+    try match goal with
+    | [ H : lc_at_var _ _ |- _ ] => inversions H
+    end;
+    repeat constructor;
+    try match goal with
+        | [ H : _ -> _ |- _ ] => eapply H; try eassumption
+        end;
+    omega.
+Qed.*)
+
+Lemma lc_at_relaxing_trm_val_def_defs:
+  (forall t k j, lc_at_trm k t -> j >= k -> lc_at_trm j t) /\
+  (forall v k j, lc_at_val k v -> j >= k -> lc_at_val j v) /\
+  (forall d k j, lc_at_def k d -> j >= k -> lc_at_def j d) /\
+  (forall ds k j, lc_at_defs k ds -> j >= k -> lc_at_defs j ds).
+Proof. Admitted. (*
+  apply trm_mutind; intros; simpl; auto;
+    match goal with
+    | [ H : lc_at_trm _ _ |- _ ] => inversions H
+    | [ H : lc_at_val _ _ |- _ ] => inversions H
+    | [ H : lc_at_def _ _ |- _ ] => inversions H
+    | [ H : lc_at_defs _ _ |- _ ] => inversions H
+    | [ H : lc_at_typ _ _ |- _ ] => inversions H
+    end;
+    repeat match goal with
+           | [ H : lc_at_var _ _ |- _ ] => inversions H
+           end;
+    repeat constructor;
+    try eapply lc_at_relaxing_typ_dec; try eassumption;
+    try match goal with
+        | [ H : _ -> _ |- _ ] => eapply H; try eassumption
+        end;
+    omega.
+Qed.*)
+
+
+Lemma lc_at_to_open_avar : forall x v k,
+    lc_at_var (S k) v -> lc_at_var k (open_rec_avar k x v).
+Proof with auto.
+  intros. inversion H; subst; repeat constructor.
+  simpl. case_if...
+  constructor. omega.
+Qed.
+
+
+Lemma lc_at_to_open_typ_dec : forall x,
+    (forall T k, lc_at_typ (S k) T -> lc_at_typ k (open_rec_typ k x T)) /\
+    (forall D k, lc_at_dec (S k) D -> lc_at_dec k (open_rec_dec k x D)).
+Proof.
+  intro x. Admitted. (*
+  apply typ_mutind; intros; simpl; auto;
+    match goal with
+    | [ H : lc_at_typ (S _) _ |- _ ] => inversions H
+    | [ H : lc_at_dec (S _) _ |- _ ] => inversions H
+    end;
+    try solve [constructor; try fold open_rec_dec; try fold open_rec_typ; auto];
+    solve [repeat constructor; apply lc_at_to_open_avar; auto].
+Qed.*)
+
+
+Lemma lc_at_to_open_trm_val_def_defs : forall x,
+    (forall t k, lc_at_trm (S k) t -> lc_at_trm k (open_rec_trm k x t)) /\
+    (forall v k, lc_at_val (S k) v -> lc_at_val k (open_rec_val k x v)) /\
+    (forall d k, lc_at_def (S k) d -> lc_at_def k (open_rec_def k x d)) /\
+    (forall ds k, lc_at_defs (S k) ds -> lc_at_defs k (open_rec_defs k x ds)).
+Proof.
+  intro x. Admitted. (*
+  apply trm_mutind; intros; simpl; auto;
+    match goal with
+    | [ H : lc_at_trm (S _) _ |- _ ] => inversions H
+    | [ H : lc_at_val (S _) _ |- _ ] => inversions H
+    | [ H : lc_at_def (S _) _ |- _ ] => inversions H
+    | [ H : lc_at_defs (S _) _ |- _ ] => inversions H
+    | [ H : lc_at_typ (S _) _ |- _ ] => inversions H
+    end;
+    repeat constructor; auto;
+    try solve [try fold open_rec_trm; auto];
+    try solve [apply lc_at_to_open_typ_dec; auto];
+    solve [apply lc_at_to_open_avar; auto].
+Qed.*)
+
+
+Lemma open_to_lc_at_avar : forall x v k,
+    lc_at_var k (open_rec_avar k x v) ->
+    lc_at_var (S k) v.
+Proof.
+  intros. inversion H; subst;
+      destruct v; simpl in *;
+        try case_if; subst; repeat constructor; auto.
+  inversion H0. omega.
+Qed.
+
+
+Lemma open_to_lc_at_typ_dec : forall x,
+    (forall T k, lc_at_typ k (open_rec_typ k x T) -> lc_at_typ (S k) T) /\
+    (forall D k, lc_at_dec k (open_rec_dec k x D) -> lc_at_dec (S k) D).
+Proof with eauto.
+  intro x. Admitted. (*
+  apply typ_mutind; intros; simpl; auto;
+    match goal with
+    | [ H : lc_at_typ _ _ |- _ ] => inversions H
+    | [ H : lc_at_dec _ _ |- _ ] => inversions H
+    end;
+    repeat constructor; auto;
+      eapply open_to_lc_at_avar...
+Qed.*)
+
+
+Lemma open_to_lc_at_trm_val_def_defs : forall x,
+    (forall t k, lc_at_trm k (open_rec_trm k x t) -> lc_at_trm (S k) t) /\
+    (forall v k, lc_at_val k (open_rec_val k x v) -> lc_at_val (S k) v) /\
+    (forall d k, lc_at_def k (open_rec_def k x d) -> lc_at_def (S k) d) /\
+    (forall ds k, lc_at_defs k (open_rec_defs k x ds) -> lc_at_defs (S k) ds).
+Proof.
+  intro x. Admitted. (*
+  apply trm_mutind; intros; simpl;
+    match goal with
+    | [ H : lc_at_trm _ _ |- _ ] => inversions H
+    | [ H : lc_at_val _ _ |- _ ] => inversions H
+    | [ H : lc_at_def _ _ |- _ ] => inversions H
+    | [ H : lc_at_defs _ _ |- _ ] => inversions H
+    | [ H : lc_at_typ _ _ |- _ ] => inversions H
+    end;
+    repeat constructor; auto;
+    try solve [try fold open_rec_trm; auto];
+    first [eapply open_to_lc_at_typ_dec | eapply open_to_lc_at_avar]; eauto.
+Qed.*)
+
+
+Lemma open_left_inverse_close_avar:
+  forall v x k, lc_at_var k v -> open_rec_avar k x (close_rec_avar k x v) = v.
+Proof with auto.
+  intros. unfold open_rec_avar, close_rec_avar.
+  inversion H; repeat case_if; subst...
+  omega.
+Qed.
+Hint Resolve open_left_inverse_close_avar.
+
+
+Lemma open_left_inverse_close_typ_dec:
+  (forall T x k, lc_at_typ k T -> open_rec_typ k x (close_rec_typ k x T) = T) /\
+  (forall D x k, lc_at_dec k D -> open_rec_dec k x (close_rec_dec k x D) = D).
+Proof with auto.
+  apply typ_mutind; intros; simpl in *; auto;
+  match goal with
+  | [ H : lc_at_typ _ _ |- _ ] => inversions H
+  | [ H : lc_at_dec _ _ |- _ ] => inversions H
+  end;
+  try apply func_eq_2;
+  try apply func_eq_1... Admitted.
+
+
+Lemma open_left_inverse_close_trm_val_def_defs :
+  (forall t k x, lc_at_trm k t -> open_rec_trm k x (close_rec_trm k x t) = t) /\
+  (forall v k x, lc_at_val k v -> open_rec_val k x (close_rec_val k x v) = v) /\
+  (forall d k x, lc_at_def k d -> open_rec_def k x (close_rec_def k x d) = d) /\
+  (forall ds k x, lc_at_defs k ds -> open_rec_defs k x (close_rec_defs k x ds) = ds).
+Proof. Admitted. (*
+  apply trm_mutind; intros; simpl in *; auto;
+    match goal with
+    | [ H : lc_at_trm _ _ |- _ ] => inversions H
+    | [ H : lc_at_val _ _ |- _ ] => inversions H
+    | [ H : lc_at_def _ _ |- _ ] => inversions H
+    | [ H : lc_at_defs _ _ |- _ ] => inversions H
+    end;
+    try apply func_eq_2;
+    try apply func_eq_1; auto;
+      apply open_left_inverse_close_typ_dec; auto.
+Qed.*)
+
+
+(** The following [lc_at_opening_XYZ] lemmas state that opening a locally
+    closed symbol (variables, types, terms, etc.) at any index
+    results in the same symbol. *)
+
+(** - variables *)
+Lemma lc_at_opening_avar: forall m n x y,
+    n >= m ->
+    lc_at_var m y ->
+    open_rec_avar n x y = y.
+Proof.
+  introv Hge Hl. inversion Hl; simpls~.
+  case_if~. omega.
+Qed.
+
+
+(** - types and declarations *)
+Lemma lc_at_opening_typ_dec: forall x m,
+    (forall T, lc_at_typ m T -> forall n, n >= m -> open_rec_typ n x T = T) /\
+    (forall D, lc_at_dec m D -> forall n, n >= m -> open_rec_dec n x D = D).
+Proof.
+  Local Hint Resolve lc_at_opening_avar.
+  intro x. Admitted. (*apply lc_at_typ_mutind; intros; simpls; f_equal*;
+  match goal with
+  | [ H : _ -> _ -> open_rec_typ _ _ _ = _ |- _ ] => apply H
+  end; omega.
+Qed.*)
+
+
+(** - terms, values, definitions, and list of definitions *)
+Lemma lc_at_opening_trm_val_def_defs: forall x m,
+  (forall t, lc_at_trm m t -> forall n, n >= m -> open_rec_trm n x t = t) /\
+  (forall v, lc_at_val m v -> forall n, n >= m -> open_rec_val n x v = v) /\
+  (forall d, lc_at_def m d -> forall n, n >= m -> open_rec_def n x d = d) /\
+  (forall ds, lc_at_defs m ds -> forall n, n >= m -> open_rec_defs n x ds = ds).
+Proof.
+  Local Hint Resolve lc_at_opening_avar.
+  intro x. Admitted. (*
+  apply lc_at_mutind; intros; simpls; f_equal*;
+    try solve
+        [match goal with
+         | [ H : _ -> _ -> ?f _ _ ?t = ?t |- ?f _ _ ?t = ?t ] => apply H
+         end; omega];
+  eapply lc_at_opening_typ_dec;
+    try eassumption;
+    try omega.
+Qed.*)
+
+
+(** The [lc_at_opening_trm_val_def_defs] lemma, specialized to terms. *)
+Lemma lc_at_opening : forall t n x,
+    lc_trm t ->
+    open_rec_trm n x t = t.
+Proof.
+  intros. eapply lc_at_opening_trm_val_def_defs; try eassumption; try omega.
+Qed.
+
+(** When a binding is removed from a locally closed evaluation context, the
+    resulting evaluation context and the value in the binding are both
+    locally closed. *)
+Lemma lc_ec_push_inv : forall s x v,
+    lc_ec (s & x ~ v) ->
+    lc_ec s /\ lc_val v.
+Proof.
+  intros s x v H.
+  inversion H.
+  - destruct (empty_push_inv H1).
+  - destruct (eq_push_inv H0) as [? [? ?] ]; subst.
+    auto.
+Qed.
+
+
+(** Values in a locally closed evaluation context are also locally closed. *)
+Lemma lc_ec_binds_inv : forall e x v,
+    lc_ec e ->
+    binds x v e ->
+    lc_val v.
+Proof.
+  intros.
+  induction e using env_ind.
+  - destruct (binds_empty_inv H0).
+  - destruct (binds_push_inv H0) as [[? ?] | [? ?]]; subst.
+    + apply (lc_ec_push_inv H).
+    + apply IHe; auto.
+      apply (lc_ec_push_inv H).
+Qed.
+
+
+(** A definition in a locally closed list of definitions is also
+    locally closed. *)
+Lemma lc_defs_has : forall ds d,
+    lc_defs ds ->
+    defs_has ds d ->
+    lc_def d.
+Proof.
+  intros.
+  induction ds.
+  - inversion H0.
+  - unfold defs_has in H0; simpl in H0.
+    cases_if.
+    + inversions H0. inversion H; auto.
+    + apply IHds; auto. inversion H; auto.
+Qed.
+
+Lemma open_bound_lc_trm : forall k x t,
+    lc_trm (open_trm x t) ->
+    open_rec_trm (S k) x t = t.
+Proof.
+  intros.
+  apply lc_at_opening with (n:=S k) (x:=x) in H.
+  eapply (proj1 (lc_open_rec_open_trm_val_def_defs x _)).
+  - instantiate (1 := 0). auto.
+  - eassumption.
+Qed.
+
+(** If [x] is closed in [t], then [x \notin fv(t)]. *)
+
+(** - for types and declarations *)
+Lemma close_rec_typ_dec_no_capture : forall x,
+    (forall T k, x \notin fv_typ (close_rec_typ k x T)) /\
+    (forall D k, x \notin fv_dec (close_rec_dec k x D)).
+Proof.
+  intros x. Admitted. (*
+  apply typ_mutind; intros; simpl; auto;
+    match goal with
+    | [ |- _ \notin fv_avar (close_rec_avar _ _ ?a) ] => destruct a
+    end; simpl;
+      try case_if; unfold fv_avar; auto.
+Qed.*)
+
+(** - for terms, values, and definitions *)
+Lemma close_rec_trm_val_def_defs_no_capture: forall x,
+    (forall t k, x \notin fv_trm (close_rec_trm k x t)) /\
+    (forall v k, x \notin fv_val (close_rec_val k x v)) /\
+    (forall d k, x \notin fv_def (close_rec_def k x d)) /\
+    (forall ds k, x \notin fv_defs (close_rec_defs k x ds)).
+Proof.
+  intro x.
+  apply trm_mutind; intros; simpl; auto;
+    try apply notin_union;
+    repeat split;
+    try apply close_rec_typ_dec_no_capture;
+    repeat
+      match goal with
+      | [ |- _ \notin fv_avar (close_rec_avar _ _ ?a) ] => destruct a; simpl
+      end;
+    repeat case_if; unfold fv_avar; auto. Admitted.
+
+(** * Free Variables Lemmas *)
+
+Lemma fv_ctx_types_push_eq : forall G x T,
+    fv_ctx_types (G & x ~ T) = fv_ctx_types G \u fv_typ T.
+Proof.
+  intros.
+  rewrite concat_def, single_def.
+  unfold fv_ctx_types, fv_in_values; rewrite values_def.
+  rewrite union_comm. reflexivity.
+Qed.
+
+(** [fv(e, x = v) = fv(e) ∪ fv(v)] *)
+Lemma fv_ec_vals_push_eq : forall e x v,
+    fv_ec_vals (e & x ~ v) = fv_ec_vals e \u fv_val v.
+Proof.
+  intros.
+  rewrite concat_def, single_def.
+  unfold fv_ec_vals, fv_in_values; rewrite values_def.
+  rewrite union_comm. reflexivity.
+Qed.
+
+(** [e(y) = v]       #<br>#
+    [x \notin fv(e)] #<br>#
+    [――――――――――――――] #<br>#
+    [x \notin fv(v)] *)
+Lemma binds_fv_ec_vals : forall x y v e,
+    binds y v e ->
+    x \notin fv_ec_vals e ->
+    x \notin fv_val v.
+Proof.
+  intros. unfold fv_ec_vals in H0.
+  eapply fv_in_values_binds; eauto.
+Qed.
+
+(** * Variable Substitution Lemmas *)
+
+(** [e(b) = v]            #<br>#
+    [――――――――――――――――――]  #<br>#
+    [e[y/x](b) = v[y/x]]  *)
+Lemma binds_subst_env : forall x y b v e,
+    binds b v e -> binds b (subst_val x y v) (subst_env x y e).
+Proof.
+  introv. gen x y b v. induction e using env_ind; intros.
+  - destruct (binds_empty_inv H).
+  - apply binds_push_inv in H.
+    destruct_all; subst; unfold subst_env; rewrite map_push.
+    + auto.
+    + apply binds_push_neq; auto.
+Qed.
+
+(** Substitution preserves local closure. *)
+
+(** - for variables *)
+(*Lemma lc_at_subst_avar : forall v x y k,
+    lc_at_var k v <-> lc_at_var k (subst_avar x y v).
+Proof.
+  intros.
+  split; intros;
+    try solve [inversion H; simpls; auto].
+  destruct v; auto.
+Qed.
+*)
+(** - for types and declarations *)
+Lemma lc_at_subst_typ_dec : forall k,
+  (forall T, lc_at_typ k T -> forall x y, lc_at_typ k (subst_typ x y T)) /\
+  (forall D, lc_at_dec k D -> forall x y, lc_at_dec k (subst_dec x y D)).
+Proof.
+  apply lc_at_typ_mutind; intros; simpls; auto.
+  constructor. Admitted. (*apply lc_at_subst_avar. trivial.*)
+
+(** - for terms, values, and definitions *)
+Lemma lc_at_subst_trm_val_def_defs : forall k,
+    (forall t, lc_at_trm k t -> forall x y, lc_at_trm k (subst_trm x y t)) /\
+    (forall v, lc_at_val k v -> forall x y, lc_at_val k (subst_val x y v)) /\
+    (forall d, lc_at_def k d -> forall x y, lc_at_def k (subst_def x y d)) /\
+    (forall ds, lc_at_defs k ds -> forall x y, lc_at_defs k (subst_defs x y ds)).
+Proof.
+  apply lc_at_mutind; intros; simpls; auto;
+    repeat constructor;
+    try solve [apply lc_at_subst_avar; trivial];
+    try apply lc_at_subst_typ_dec; trivial.
+Admitted.
+
+(** * Lemmas *)
+
+(** The following [subst_fresh_XYZ] lemmas state that if [x] is not free
+    in a symbol [Y], then [Y[z/x] = Y]. *)
+
+(** Fresh substitution
+    - in variables *)
+Lemma subst_fresh_avar: forall x y,
+  (forall a: avar, x \notin fv_avar a -> subst_avar x y a = p_sel a nil).
+Proof.
+  intros. destruct* a. simpl. autounfold. case_var*. simpls. notin_false.
+Qed.
+
+Lemma subst_fresh_path : forall x q p,
+    x \notin fv_path p ->
+    subst_path x q p = p.
+Proof.
+  intros. destruct p as [[n | z] bs]; simpls.
+  - Case "p = (avar_b n).bs".
+    rewrite* app_nil_r.
+  - Case "p = (avar_f z).bs".
+    unfold subst_var_p. apply notin_singleton in H. case_if.
+    simpl. rewrite* app_nil_r.
+Qed.
+
+(** - in types, declarations, paths *)
+Lemma subst_fresh_typ_dec: forall x y,
+  (forall T : typ  , x \notin fv_typ  T  -> subst_typ  x y T  = T ) /\
+  (forall D : dec  , x \notin fv_dec  D  -> subst_dec  x y D  = D ).
+Proof.
+  intros x y. apply typ_mutind; intros; simpls; f_equal*. apply* subst_fresh_path.
+Qed.
+
+Definition subst_fresh_typ x p := proj1 (subst_fresh_typ_dec x p).
+
+(** - in terms, values, and definitions *)
+Lemma subst_fresh_trm_val_def_defs: forall x y,
+  (forall t : trm , x \notin fv_trm  t  -> subst_trm  x y t  = t ) /\
+  (forall v : val , x \notin fv_val  v  -> subst_val  x y v  = v ) /\
+  (forall d : def , x \notin fv_def  d  -> subst_def  x y d  = d ) /\
+  (forall ds: defs, x \notin fv_defs ds -> subst_defs x y ds = ds).
+Proof.
+  intros x y. apply trm_mutind; intros; simpls; f_equal*;
+    (apply* subst_fresh_typ_dec || apply* subst_fresh_path).
+Qed.
+
+Lemma fv_ctx_types_concat_eq : forall G1 G2,
+    fv_ctx_types (G1 & G2) = fv_ctx_types G1 \u fv_ctx_types G2.
+Proof.
+  intros G1 G2. induction G2 using env_ind.
+  - unfold fv_ctx_types, fv_in_values; rewrite values_def.
+    rewrite concat_empty_r, empty_def, union_empty_r; reflexivity.
+  - rewrite concat_assoc. rewrite fv_ctx_types_push_eq.
+    rewrite IHG2. rewrite <- union_assoc. f_equal.
+    symmetry. apply fv_ctx_types_push_eq.
+Qed.
+
+Lemma notin_fv_ctx_concat : forall x G2 G1,
+    x \notin fv_ctx_types (G1 & G2) <->
+    x \notin fv_ctx_types G1 /\ x \notin fv_ctx_types G2.
+Proof.
+  intros. rewrite <- notin_union.
+  rewrite <- fv_ctx_types_concat_eq.
+  split; intros; assumption.
+Qed.
+
+(** [x \notin fv(T)]           #<br>#
+    [x \notin fv(G)]       #<br>#
+    [―――――――――――――――――――――――] #<br>#
+    [x \notin fv(G, z: T)] *)
+Lemma fv_ctx_types_push: forall x z T G,
+    x \notin fv_typ T ->
+    x \notin fv_ctx_types G ->
+    x \notin fv_ctx_types (G & z ~ T).
+Proof.
+  intros. rewrite fv_ctx_types_push_eq.
+  apply notin_union. split~.
+Qed.
+
+(** [x \notin fv(G, z: T)]                   #<br>#
+    [x \notin fv(T)]                         #<br>#
+    [―――――――――――――――――――――――――――――――――――――] #<br>#
+    [x \notin fv(T)] and [x \notin fv(G)] *)
+Lemma invert_fv_ctx_types_push: forall x z T G,
+  x \notin fv_ctx_types (G & z ~ T) -> x \notin fv_typ T /\ x \notin (fv_ctx_types G).
+Proof.
+  introv H. rewrite fv_ctx_types_push_eq in H.
+  apply~ notin_union.
+Qed.
+
+(** [x \notin fv(G)]         #<br>#
+    [――――――――――――――――――]    #<br>#
+    [G[y/x] = G]    *)
+Lemma subst_fresh_ctx: forall x y G,
+  x \notin fv_ctx_types G -> subst_ctx x y G = G.
+Proof.
+  intros x y.
+  apply (env_ind (fun G => x \notin fv_ctx_types G -> subst_ctx x y G = G)).
+  + intro N. unfold subst_ctx. apply map_empty.
+  + intros G z T IH N.
+    apply invert_fv_ctx_types_push in N. destruct N as [N1 N2].
+    unfold subst_ctx in *. rewrite map_push.
+    rewrite (IH N2).
+    rewrite ((proj1 (subst_fresh_typ_dec _ _)) _ N1).
+    reflexivity.
+Qed.
+(*
+(** Definition of substitution on named variables: #<br>#
+    [z[y/x] := if z == x then y else z], where [z] is a named variable. *)
+Definition subst_fvar(x y z: var): var := If z = x then y else z.*)
+
+(** The following lemmas state that substitution commutes with opening:
+    for a symbol [Z], #<br>#
+    [(Z^a)[y/x] = (Z[y/x])^(a[y/x])]. *)
+
+(** Substitution commutes with opening
+    - variables *)
+Lemma subst_open_commut: forall x p u y n,
+    lc_path p ->
+    subst_avar x p (open_rec_avar n u y)
+    = open_rec_path_p n (subst_var_p x p u) (subst_avar x p y).
+Proof.
+  introv Hl. unfold subst_var_p, subst_avar, open_rec_avar, subst_var_p.
+  destruct y as [n' | y]; autounfold; destruct p as [z bs]; destruct z as [m | z'];
+    repeat case_if; simpl; try case_if*; eauto; inversions  Hl; inversions H0. Admitted.
+
+Lemma sel_fields_open : forall n p q bs,
+  sel_fields (open_rec_path_p n p q) bs = open_rec_path_p n p (sel_fields q bs).
+Proof.
+  intros. destruct q. simpl. destruct p. destruct a. case_if; simpl; auto. rewrite* app_assoc.
+  simpl. auto.
+Qed.
+
+Lemma sel_fields_subst : forall x p y bs b,
+    subst_path x p (p_sel y bs) • b = (subst_path x p (p_sel y bs)) • b.
+Proof.
+  intros. destruct p, y; auto. simpl. unfold subst_var_p. case_if; simpl; auto.
+Qed.
+
+(** - paths *)
+Lemma subst_open_commut_path: forall p n x q u,
+    lc_path p ->
+    subst_path x p (open_rec_path n u q)
+    = open_rec_path_p n (subst_var_p x p u) (subst_path x p q).
+Proof.
+  introv Hl. destruct q as [z bs]. simpl. rewrite* subst_open_commut. rewrite* sel_fields_open.
+Qed.
+
+(** - types and declarations *)
+Lemma subst_open_commut_typ_dec: forall x p u,
+  lc_path p ->
+  (forall t : typ, forall n: nat,
+     subst_typ x p (open_rec_typ n u t)
+     = open_rec_typ_p n (subst_var_p x p u) (subst_typ x p t)) /\
+  (forall D : dec, forall n: nat,
+     subst_dec x p (open_rec_dec n u D)
+     = open_rec_dec_p n (subst_var_p x p u) (subst_dec x p D)).
+Proof.
+  intros. apply typ_mutind; intros; simpl; f_equal*. apply* subst_open_commut_path.
+Qed.
+
+Lemma subst_open_commut_p: forall x p u y n,
+    lc_path p ->
+    subst_path x p (open_rec_avar_p n u y)
+    = open_rec_path_p n (subst_path x p u) (subst_avar x p y).
+Proof.
+  introv Hl. unfold subst_path, subst_avar, subst_var_p.
+  destruct y as [n' | y]; simpl; repeat case_if; destruct u; destruct a; simpl;
+    try (rewrite* app_nil_r); repeat case_if; unfold sel_fields; destruct* p;
+      inversions Hl; inversions H0; rewrite* app_nil_l.
+Admitted.
+
+Lemma subst_open_commut_path_p: forall p n x q u,
+    lc_path q ->
+    subst_path x q (open_rec_path_p n u p)
+    = open_rec_path_p n (subst_path x q u) (subst_path x q p).
+Proof.
+  introv Hl. destruct p as [z bs]. simpl.
+  unfold subst_path. destruct u. rewrite <- sel_fields_open.
+  unfold open_rec_path_p, subst_avar.
+  destruct z; simpl; destruct a; repeat case_if*;
+    unfold subst_var_p; repeat case_if;
+      destruct q; simpl; try (rewrite app_assoc || rewrite app_nil_r);
+        try solve [inversion Hl; inversion* H0].
+Admitted.
+
+Lemma subst_open_commut_typ_dec_p: forall x y u,
+  lc_path y ->
+  (forall t : typ, forall n: nat,
+     subst_typ x y (open_rec_typ_p n u t)
+     = open_rec_typ_p n (subst_path x y u) (subst_typ x y t)) /\
+  (forall D : dec, forall n: nat,
+     subst_dec x y (open_rec_dec_p n u D)
+     = open_rec_dec_p n (subst_path x y u) (subst_dec x y D)).
+Proof.
+  intros. apply typ_mutind; intros; simpl; f_equal*.
+  apply* subst_open_commut_path_p.
+Qed.
+
+(** - types only *)
+Lemma subst_open_commut_typ: forall x y u T,
+  lc_path y ->
+  subst_typ x y (open_typ u T) = open_typ_p (subst_var_p x y u) (subst_typ x y T).
+Proof.
+  intros. apply* subst_open_commut_typ_dec.
+Qed.
+
+Lemma subst_open_commut_typ_p: forall x y u T,
+    lc_path y ->
+    subst_typ x y (open_typ_p u T) = open_typ_p (subst_path x y u) (subst_typ x y T).
+Proof.
+  intros. apply* subst_open_commut_typ_dec_p.
+Qed.
+
+(** - terms, values, definitions, and list of definitions *)
+Lemma subst_open_commut_trm_val_def_defs: forall x y u,
+    lc_path y ->
+  (forall t : trm, forall n: nat,
+     subst_trm x y (open_rec_trm n u t)
+     = open_rec_trm_p n (subst_var_p x y u) (subst_trm x y t)) /\
+  (forall v : val, forall n: nat,
+     subst_val x y (open_rec_val n u v)
+     = open_rec_val_p n (subst_var_p x y u) (subst_val x y v)) /\
+  (forall d : def , forall n: nat,
+     subst_def x y (open_rec_def n u d)
+     = open_rec_def_p n (subst_var_p x y u) (subst_def x y d)) /\
+  (forall ds: defs, forall n: nat,
+     subst_defs x y (open_rec_defs n u ds)
+     = open_rec_defs_p n (subst_var_p x y u) (subst_defs x y ds)).
+Proof.
+  intros. apply trm_mutind; intros; simpl; f_equal*;
+  apply* subst_open_commut_path || apply* subst_open_commut_typ_dec.
+Qed.
+
+Lemma subst_open_commut_trm_val_def_defs_p: forall x y u,
+    lc_path y ->
+  (forall t : trm, forall n: nat,
+     subst_trm x y (open_rec_trm_p n u t)
+     = open_rec_trm_p n (subst_path x y u) (subst_trm x y t)) /\
+  (forall v : val, forall n: nat,
+     subst_val x y (open_rec_val_p n u v)
+     = open_rec_val_p n (subst_path x y u) (subst_val x y v)) /\
+  (forall d : def , forall n: nat,
+     subst_def x y (open_rec_def_p n u d)
+     = open_rec_def_p n (subst_path x y u) (subst_def x y d)) /\
+  (forall ds: defs, forall n: nat,
+     subst_defs x y (open_rec_defs_p n u ds)
+     = open_rec_defs_p n (subst_path x y u) (subst_defs x y ds)).
+Proof.
+  intros. apply trm_mutind; intros; simpl; f_equal*;
+  apply* subst_open_commut_typ_dec_p || apply* subst_open_commut_path_p.
+Qed.
+
+(** - terms only *)
+Lemma subst_open_commut_trm: forall x y u t,
+    lc_path y ->
+    subst_trm x y (open_trm u t)
+    = open_trm_p (subst_var_p x y u) (subst_trm x y t).
+Proof.
+  intros. apply* subst_open_commut_trm_val_def_defs.
+Qed.
+
+Lemma subst_open_commut_trm_p: forall x y u t,
+    lc_path y ->
+    subst_trm x y (open_trm_p u t)
+    = open_trm_p (subst_path x y u) (subst_trm x y t).
+Proof.
+  intros. apply* subst_open_commut_trm_val_def_defs_p.
+Qed.
+
+(** - definitions only *)
+Lemma subst_open_commut_defs: forall x y u ds,
+    lc_path y ->
+    subst_defs x y (open_defs u ds)
+    = open_defs_p (subst_var_p x y u) (subst_defs x y ds).
+Proof.
+  intros. apply* subst_open_commut_trm_val_def_defs.
+Qed.
+
+Lemma subst_open_commut_defs_p: forall x y u ds,
+    lc_path y ->
+    subst_defs x y (open_defs_p u ds)
+    = open_defs_p (subst_path x y u) (subst_defs x y ds).
+Proof.
+  intros. apply* subst_open_commut_trm_val_def_defs_p.
+Qed.
+
+(** The following lemmas state that opening a symbol with a variable [y]
+    is the same as opening the symbol with another variable [x] and
+    substituting [x] with [y]: #<br>#
+    [Z^y = (Z^x)[y/x]] *)
+
+(** Substitution after opening
+    - terms *)
+Lemma subst_intro_trm: forall x u t, x \notin (fv_trm t) -> lc_path u ->
+  open_trm_p u t = subst_trm x u (open_trm x t).
+Proof.
+  introv Fr Hl. unfold open_trm. rewrite* subst_open_commut_trm.
+  destruct (@subst_fresh_trm_val_def_defs x u) as [Q _]. rewrite~ (Q t).
+  unfold subst_var_p. case_var~.
+Qed.
+
+(** - definitions *)
+Lemma subst_intro_defs: forall x u ds, x \notin (fv_defs ds) -> lc_path u ->
+  open_defs_p u ds = subst_defs x u (open_defs x ds).
+Proof.
+  introv Fr Hl. unfold open_trm. rewrite* subst_open_commut_defs.
+  destruct (@subst_fresh_trm_val_def_defs x u) as [_ [_ [_ Q]]]. rewrite~ (Q ds).
+  unfold subst_var_p. case_var~.
+Qed.
+
+(** - types *)
+Lemma subst_intro_typ: forall x u T, x \notin (fv_typ T) -> lc_path u ->
+  open_typ_p u T = subst_typ x u (open_typ x T).
+Proof.
+  introv Fr Hl. unfold open_typ. rewrite* subst_open_commut_typ.
+  destruct (@subst_fresh_typ_dec x u) as [Q _]. rewrite* (Q T).
+  unfold subst_var_p. case_var*.
+Qed.
+
+Ltac subst_open_fresh :=
+  match goal with
+  | [ |- context [ open_typ ?z (subst_typ ?x ?p ?T) ] ] =>
+    replace (open_typ z (subst_typ x p T)) with (open_typ_p (subst_path x p (pvar z)) (subst_typ x p T)) by
+        (unfold subst_path; simpl; unfold subst_var_p; rewrite If_r, open_var_typ_eq; auto)
+    | [ |- context [ open_defs ?z (subst_defs ?x ?p ?ds) ] ] =>
+        replace (open_defs z (subst_defs x p ds)) with (open_defs_p (subst_path x p (pvar z)) (subst_defs x p ds))
+          by (unfold subst_path; simpl; unfold subst_var_p; rewrite If_r, open_var_defs_eq; auto)
+     | [ |- context [ open_trm ?z (subst_trm ?x ?p ?t) ] ] =>
+        replace (open_trm z (subst_trm x p t)) with (open_trm_p (subst_path x p (pvar z)) (subst_trm x p t))
+          by (unfold subst_path; simpl; unfold subst_var_p; rewrite If_r, open_var_trm_eq; auto)
+    end.
+
+(** Substitution preserves labels of definitions: [label(d) = label(d[y/x])] *)
+Lemma subst_label_of_def: forall x y d,
+  label_of_def d = label_of_def (subst_def x y d).
+Proof.
+  intros. destruct* d.
+Qed.
+
+(** [l \notin labels(ds)]     #<br>#
+    [――――――――――――――――――――――] #<br>#
+    [l \notin labels(ds[y/x]] *)
+Lemma subst_defs_hasnt: forall x y l ds,
+  defs_hasnt ds l ->
+  defs_hasnt (subst_defs x y ds) l.
+Proof.
+  intros x y l ds. unfold defs_hasnt. induction ds; introv Eq; auto.
+  unfold get_def. simpl. rewrite <- subst_label_of_def.
+  simpl in Eq. case_if~.
+Qed.
+
+(** Definition of substitution on named variables: #<br>#
+    [z[y/x] := if z == x then y else z], where [z] is a named variable. *)
+Definition subst_fvar(x y z: var): var := If z = x then y else z.
+
+
+(** [z <> x]                             #<br>#
+    [ds^z = ...{a = t}...]              #<br>#
+    [――――――――――――――――――――――――――――――――]  #<br>#
+    [(ds[y/x])^z = ...{a = t[y/x]}...]  *)
+Lemma open_subst_defs : forall x y z a ds t,
+    z <> x ->
+    defs_has (open_defs z ds) (def_trm a t) ->
+    defs_has (open_defs z (subst_defs x y ds)) (def_trm a (subst_trm x y t)).
+Proof.
+  introv. gen x y z a t. induction ds; intros.
+  - inversion H0.
+  - unfold open_defs, defs_has in *; simpls. case_if.
+    + destruct d; simpls; case_if; auto.
+      inversions H0.
+      rewrite subst_open_commut_trm. unfold subst_fvar.
+      Admitted. (*case_if. auto.
+    + case_if; apply IHds; destruct d; auto; contradiction.
+Qed.*)
+
+(** [y <> x]                             #<br>#
+    [ds^x = ...{a = t}...]              #<br>#
+    [――――――――――――――――――――――――――――――――]  #<br>#
+    [(ds[y/x])^y = ...{a = t[y/x]}...]  *)
+(*Lemma open_subst_defs2 : forall x y a ds t,
+    y <> x ->
+    defs_has (open_defs x ds) (def_trm a t) ->
+    defs_has (open_defs y (subst_defs x y ds)) (def_trm a (subst_trm x y t)).
+Proof.
+  introv. gen x y a t. induction ds; intros.
+  - inversion H0.
+  - unfold open_defs, defs_has in *.
+    simpls; case_if; destruct d; simpls; case_if; auto.
+    subst; inversion H0.
+    rewrite subst_open_commut_trm. unfold subst_fvar. case_if; auto.
+Qed.
+*)
